define a more generic heap field assignment rule from which the instantiated rule is derived from

viper-total-heaps/StmtRel.thy
@@ -344,6 +344,101 @@ qed (insert assms, simp_all)
 
 subsection \<open>Field assignment relation\<close>
 
+definition field_assign_normal_premise
+  where "field_assign_normal_premise ctxt StateCons e_r f e \<omega> addr v ty \<equiv> 
+    ctxt, StateCons, (Some \<omega>) \<turnstile> \<langle>e_r; \<omega>\<rangle> [\<Down>]\<^sub>t Val (VRef (Address addr)) \<and>
+    (addr,f) \<in> get_writeable_locs \<omega> \<and>
+    ctxt, StateCons, (Some \<omega>)  \<turnstile> \<langle>e; \<omega>\<rangle> [\<Down>]\<^sub>t Val v \<and>
+    declared_fields (program_total ctxt) f = Some ty \<and>
+    get_type (absval_interp_total ctxt) v = ty"
+
+lemma field_assign_rel_general:
+  assumes SubExpsWfRel: "exprs_wf_rel (rel_ext_eq R) ctxt_vpr StateCons P ctxt [rcv_vpr,rhs_vpr] \<gamma> \<gamma>1"
+      and WriteableLocRel: "wf_rel_fieldacc get_writeable_locs (rel_ext_eq R) (rel_ext_eq R) ctxt_vpr StateCons P ctxt rcv_vpr f_vpr 
+                 \<gamma>1 \<gamma>2"
+      and UpdHeapRel: "rel_general R R (\<lambda>\<omega> \<omega>'. \<exists>\<tau>_vpr addr v. \<omega>' = update_hh_loc_total_full \<omega> (addr,f_vpr) v \<and>
+                                                       field_assign_normal_premise ctxt_vpr StateCons rcv_vpr f_vpr rhs_vpr \<omega> addr v \<tau>_vpr) (\<lambda>_. False) P ctxt \<gamma>2 \<gamma>'"
+    shows "stmt_rel R R ctxt_vpr StateCons \<Lambda>_vpr P ctxt (ViperLang.FieldAssign rcv_vpr f_vpr rhs_vpr) \<gamma> \<gamma>'"
+proof (rule stmt_rel_intro)
+  let ?Rext = "rel_ext_eq R"
+  fix \<omega> ns \<omega>'
+  assume "R \<omega> ns"
+  hence "?Rext \<omega> \<omega> ns" by simp
+
+  assume "red_stmt_total ctxt_vpr StateCons \<Lambda>_vpr (FieldAssign rcv_vpr f_vpr rhs_vpr) \<omega> (RNormal \<omega>')"
+  thus "\<exists>ns'. red_ast_bpl P ctxt (\<gamma>, Normal ns) (\<gamma>', Normal ns') \<and> R \<omega>' ns'"
+    proof cases
+      case (RedFieldAssign addr v ty_vpr)
+      hence "red_pure_exps_total ctxt_vpr StateCons (Some \<omega>) [rcv_vpr, rhs_vpr] \<omega> (Some [VRef (Address addr), v])"
+        by (auto intro!: TotalExpressions.RedExpListCons TotalExpressions.RedExpListNil)
+
+      from this obtain ns1 where
+        "?Rext \<omega> \<omega> ns1" and "red_ast_bpl P ctxt (\<gamma>, Normal ns) (\<gamma>1, Normal ns1)"
+        using exprs_wf_rel_normal_elim[OF SubExpsWfRel \<open>?Rext \<omega> \<omega> ns\<close>]
+        by blast
+      with RedFieldAssign obtain ns3 where "?Rext \<omega> \<omega> ns3" and RedNs3: "red_ast_bpl P ctxt (\<gamma>, Normal ns) (\<gamma>2, Normal ns3)" 
+        using wf_rel_normal_elim[OF WriteableLocRel] red_ast_bpl_transitive
+        by blast
+      hence "R \<omega> ns3" 
+        by simp
+  
+      have "field_assign_normal_premise ctxt_vpr StateCons rcv_vpr f_vpr rhs_vpr \<omega> addr v ty_vpr"
+        using RedFieldAssign
+        unfolding field_assign_normal_premise_def
+        by fastforce
+  
+      with rel_success_elim[OF UpdHeapRel \<open>R \<omega> ns3\<close>] obtain ns4
+        where "red_ast_bpl P ctxt (\<gamma>2, Normal ns3) (\<gamma>', Normal ns4) \<and> R \<omega>' ns4"
+        unfolding \<open>\<omega>' = _\<close>
+        by blast
+  
+      thus ?thesis
+        using RedNs3 red_ast_bpl_transitive
+        by blast     
+  qed
+next
+  let ?Rext = "rel_ext_eq R"
+  fix \<omega> ns 
+  assume "R \<omega> ns"
+  hence "?Rext \<omega> \<omega> ns" by simp
+  assume "red_stmt_total ctxt_vpr StateCons \<Lambda>_vpr (FieldAssign rcv_vpr f_vpr rhs_vpr) \<omega> RFailure"
+  thus "\<exists>c'. snd c' = Failure \<and> red_ast_bpl P ctxt (\<gamma>, Normal ns) c'"
+  proof cases
+    case (RedFieldAssignFailure r v)
+    hence "red_pure_exps_total ctxt_vpr StateCons (Some \<omega>) [rcv_vpr, rhs_vpr] \<omega> (Some [VRef r, v])"
+      by (auto intro!: TotalExpressions.RedExpListCons TotalExpressions.RedExpListNil)
+      from this obtain ns1 where
+        "?Rext \<omega> \<omega> ns1" and "red_ast_bpl P ctxt (\<gamma>, Normal ns) (\<gamma>1, Normal ns1)"
+        using exprs_wf_rel_normal_elim[OF SubExpsWfRel \<open>?Rext \<omega> \<omega> ns\<close>]
+        by blast   
+    with RedFieldAssignFailure obtain \<gamma>' where "red_ast_bpl P ctxt (\<gamma>, Normal ns) (\<gamma>', Failure)"
+      using wf_rel_failure_elim[OF WriteableLocRel \<open>?Rext \<omega> \<omega> ns1\<close>] red_ast_bpl_transitive
+      by (metis (no_types, opaque_lifting) ref.exhaust ref.sel snd_conv surj_pair)
+    thus ?thesis
+      by (meson snd_conv)
+  next
+    case RedSubExpressionFailure
+    hence RedSubExpFailureAux: "red_pure_exps_total ctxt_vpr StateCons (Some \<omega>) [rcv_vpr, rhs_vpr] \<omega> None"
+      by simp
+    thus ?thesis
+      using exprs_wf_rel_failure_elim[OF SubExpsWfRel \<open>?Rext \<omega> \<omega> ns\<close>]
+      by blast
+  qed
+qed
+
+lemma field_assign_rel_general_2:
+  assumes RcvWfRel: "expr_wf_rel (rel_ext_eq R) ctxt_vpr StateCons P ctxt rcv_vpr \<gamma> \<gamma>1"
+      and RhsWfRel: "expr_wf_rel (rel_ext_eq R) ctxt_vpr StateCons P ctxt rhs_vpr \<gamma>1 \<gamma>2"
+      and WriteableLocRel: "wf_rel_fieldacc get_writeable_locs (rel_ext_eq R) (rel_ext_eq R) ctxt_vpr StateCons P ctxt rcv_vpr f_vpr 
+                 \<gamma>2 \<gamma>3"
+      and UpdHeapRel: "rel_general R R (\<lambda>\<omega> \<omega>'. \<exists>\<tau>_vpr addr v. \<omega>' = update_hh_loc_total_full \<omega> (addr,f_vpr) v \<and>
+                                                       field_assign_normal_premise ctxt_vpr StateCons rcv_vpr f_vpr rhs_vpr \<omega> addr v \<tau>_vpr) (\<lambda>_. False) P ctxt \<gamma>3 \<gamma>'"
+    shows "stmt_rel R R ctxt_vpr StateCons \<Lambda>_vpr P ctxt (ViperLang.FieldAssign rcv_vpr f_vpr rhs_vpr) \<gamma> \<gamma>'"
+  apply (rule field_assign_rel_general[OF _ WriteableLocRel UpdHeapRel])
+  apply (rule exprs_wf_rel_alt_implies_exprs_wf_rel)
+  using RcvWfRel RhsWfRel
+  by (auto simp del: Product_Type.split_paired_Ex)
+
 lemma field_assign_rel:
   assumes WfConsistency: "wf_total_consistency ctxt_vpr StateCons StateCons_t"
       and Consistent: "StateConsEnabled \<Longrightarrow> (\<And> \<omega> ns. R \<omega> ns \<Longrightarrow> StateCons \<omega>)"
@@ -370,82 +465,78 @@ lemma field_assign_rel:
                        vbpl_absval_ty_opt TyRep (AHeap hb) = Some (THeapId TyRep, []) \<and>
                        lookup_var (var_context ctxt) ns f_bpl = Some (AbsV (AField f_bpl_val)) \<and>
                        field_ty_fun_opt TyRep f_bpl_val = Some (TFieldId TyRep, [\<tau>_field_bpl, \<tau>_bpl]) \<and>
-                       vbpl_absval_ty_opt TyRep (AHeap (hb( (Address addr,f_bpl_val) \<mapsto> (val_rel_vpr_bpl v) ))) = Some (THeapId TyRep, []) \<and>
                        R (update_hh_loc_total_full \<omega> (addr,f_vpr) v)
                          (update_var (var_context ctxt) ns h_bpl
                                (AbsV (AHeap (hb( (Address addr,f_bpl_val) \<mapsto> (val_rel_vpr_bpl v) ))))
                          ))"
   shows "stmt_rel R R ctxt_vpr StateCons \<Lambda>_vpr P ctxt (ViperLang.FieldAssign rcv_vpr f_vpr rhs_vpr) 
          \<gamma>
-         (BigBlock name cs str tr, cont)" 
-proof (rule stmt_rel_intro)
-  let ?\<gamma>3="((BigBlock name ((Lang.Assign h_bpl h_upd_bpl)#cs) str tr), cont)"
-  let ?Rext = "rel_ext_eq R"
-  fix \<omega> ns \<omega>'
-  assume "R \<omega> ns"
-  hence "?Rext \<omega> \<omega> ns" by simp
+         (BigBlock name cs str tr, cont)"   
+proof (rule field_assign_rel_general_2[OF RcvWfRel RhsWfRel WriteableLocRel])
+  show "rel_general R R
+        (\<lambda>\<omega> \<omega>'. \<exists>\<tau>_vpr addr v. \<omega>' = update_hh_loc_total_full \<omega> (addr, f_vpr) v \<and> field_assign_normal_premise ctxt_vpr StateCons rcv_vpr f_vpr rhs_vpr \<omega> addr v \<tau>_vpr) (\<lambda>_. False)
+        P ctxt (BigBlock name (Assign h_bpl h_upd_bpl # cs) str tr, cont) (BigBlock name cs str tr, cont)"
+  proof (rule rel_intro_no_fail)
+    let ?Rext = "rel_ext_eq R"
+    fix \<omega> ns \<omega>'
+    assume "R \<omega> ns"
+       and "\<exists>\<tau>_vpr addr v. \<omega>' = update_hh_loc_total_full \<omega> (addr, f_vpr) v \<and> field_assign_normal_premise ctxt_vpr StateCons rcv_vpr f_vpr rhs_vpr \<omega> addr v \<tau>_vpr"
 
-  assume RedStmt: "red_stmt_total ctxt_vpr StateCons \<Lambda>_vpr (FieldAssign rcv_vpr f_vpr rhs_vpr) \<omega> (RNormal \<omega>')"
-
-  thus "\<exists>ns'. red_ast_bpl P ctxt (\<gamma>, Normal ns) ((BigBlock name cs str tr, cont), Normal ns') \<and> R \<omega>' ns'"
-  proof cases
-    case (RedFieldAssign addr v ty_vpr)
-    from this obtain ns1 where
-      "?Rext \<omega> \<omega> ns1" and "red_ast_bpl P ctxt (\<gamma>, Normal ns) (\<gamma>1, Normal ns1)"
-      using wf_rel_normal_elim[OF RcvWfRel \<open>?Rext \<omega> \<omega> ns\<close>]
+    from this obtain \<tau>_vpr addr v
+      where "\<omega>' = update_hh_loc_total_full \<omega> (addr, f_vpr) v"
+        and FieldPremise:"field_assign_normal_premise ctxt_vpr StateCons rcv_vpr f_vpr rhs_vpr \<omega> addr v \<tau>_vpr"
       by auto
-    from this RedFieldAssign obtain ns2 where "?Rext \<omega> \<omega> ns2" and "red_ast_bpl P ctxt (\<gamma>, Normal ns) (\<gamma>2, Normal ns2)"
-      using wf_rel_normal_elim[OF RhsWfRel] red_ast_bpl_transitive
-      by blast
-    from this RedFieldAssign obtain ns3 where "?Rext \<omega> \<omega> ns3" and RedNs3: "red_ast_bpl P ctxt (\<gamma>, Normal ns) (?\<gamma>3, Normal ns3)" 
-      using wf_rel_normal_elim[OF WriteableLocRel] red_ast_bpl_transitive
-      by blast
-    hence "R \<omega> ns3" by simp
 
-    have "vpr_to_bpl_ty TyRep ty_vpr = Some \<tau>_bpl"         
-      using \<open>declared_fields _ f_vpr = Some ty_vpr\<close> DeclaredFieldsSome
+    from \<open>R \<omega> ns\<close> have "?Rext \<omega> \<omega> ns"
       by simp
- 
+   
+    note FieldPremiseSimp = FieldPremise[simplified  field_assign_normal_premise_def]
+
+    have RedStmt: "red_stmt_total ctxt_vpr StateCons \<Lambda>_vpr (FieldAssign rcv_vpr f_vpr rhs_vpr) \<omega> (RNormal \<omega>')"
+      unfolding \<open>\<omega>' = _\<close>
+      apply (rule RedFieldAssign)
+      using FieldPremiseSimp
+      by auto
+
    moreover have NewValTypeBpl: "type_of_vbpl_val TyRep (val_rel_vpr_bpl v) = \<tau>_bpl"
-     using vpr_to_bpl_val_type[OF \<open>get_type _ v = ty_vpr\<close> \<open>vpr_to_bpl_ty TyRep ty_vpr = Some \<tau>_bpl\<close>]
-           \<open>domain_type _ = _\<close>
-     by simp
+     using vpr_to_bpl_val_type FieldPremiseSimp
+           \<open>domain_type _ = _\<close> DeclaredFieldsSome
+     by fastforce
 
    moreover from RedStmt have "StateConsEnabled \<Longrightarrow> StateCons \<omega>'"
      using total_consistency_red_stmt_preserve[OF WfConsistency] Consistent[OF _ \<open>R \<omega> ns\<close>]
      by simp
 
    moreover from RedFieldAssign DomainTypeEq have "get_type (domain_type TyRep) v = \<tau>_vpr"
-     using DeclaredFieldsSome
-     by force
+     using DeclaredFieldsSome FieldPremiseSimp 
+     by presburger
 
    ultimately obtain hb f_bpl_val
      where 
            LookupTyHeapBpl: "lookup_var_ty (var_context ctxt) h_bpl = Some (TConSingle (THeapId TyRep))" and
-           LookupHeapVarBpl: "lookup_var (var_context ctxt) ns3  h_bpl = Some (AbsV (AHeap hb))" and
+           LookupHeapVarBpl: "lookup_var (var_context ctxt) ns  h_bpl = Some (AbsV (AHeap hb))" and
            HeapWellTyBpl: "vbpl_absval_ty_opt TyRep (AHeap hb) = Some (THeapId TyRep, [])" and
-           HeapUpdWellTyBpl: "vbpl_absval_ty_opt TyRep (AHeap (hb( (Address addr,f_bpl_val) \<mapsto> (val_rel_vpr_bpl v) ))) = Some (THeapId TyRep, [])" and
-           LookupFieldVarBpl: "lookup_var (var_context ctxt) ns3 f_bpl = Some (AbsV (AField f_bpl_val))" and           
+           LookupFieldVarBpl: "lookup_var (var_context ctxt) ns f_bpl = Some (AbsV (AField f_bpl_val))" and           
            FieldTyBpl: "field_ty_fun_opt TyRep f_bpl_val = Some ((TFieldId TyRep), [\<tau>_field_bpl, \<tau>_bpl])" and
            "R \<omega>'
-                   (update_var (var_context ctxt) ns3 h_bpl
+                   (update_var (var_context ctxt) ns h_bpl
                    (AbsV (AHeap (hb( (Address addr,f_bpl_val) \<mapsto> (val_rel_vpr_bpl v) ))))
              )" (is "R _ ?ns_upd")
-     using RFieldAssign[OF \<open>R \<omega> ns3\<close>] \<open>\<omega>' = _\<close>           
-     by metis
+     using RFieldAssign[OF \<open>R \<omega> ns\<close>] \<open>\<omega>' = _\<close> FieldPremiseSimp DeclaredFieldsSome
+     by fastforce
 
-   from RcvRel have RedRcvBpl: "red_expr_bpl ctxt rcv_bpl ns3 (AbsV (ARef (Address addr)))"
-     using \<open>?Rext \<omega> \<omega> ns3\<close>  RedFieldAssign exp_rel_vpr_bpl_elim
+   from RcvRel have RedRcvBpl: "red_expr_bpl ctxt rcv_bpl ns (AbsV (ARef (Address addr)))"
+     using \<open>?Rext \<omega> \<omega> ns\<close>  FieldPremiseSimp exp_rel_vpr_bpl_elim
      by (metis (mono_tags, lifting) val_rel_vpr_bpl.simps(3))
 
-   from RhsRel have RedRhsBpl: "red_expr_bpl ctxt rhs_bpl ns3 (val_rel_vpr_bpl v)" 
-     using \<open>?Rext \<omega> \<omega> ns3\<close>  RedFieldAssign exp_rel_vpr_bpl_elim
+   from RhsRel have RedRhsBpl: "red_expr_bpl ctxt rhs_bpl ns (val_rel_vpr_bpl v)" 
+     using \<open>?Rext \<omega> \<omega> ns\<close>  FieldPremiseSimp exp_rel_vpr_bpl_elim
      by (metis (mono_tags, lifting))
 
    from HeapUpdWf have 
       RedHeapUpdBpl:
      "red_expr_bpl ctxt (heap_upd_bpl (Lang.Var h_bpl) rcv_bpl (Lang.Var f_bpl) rhs_bpl [\<tau>_field_bpl, \<tau>_bpl])
-                             ns3 (AbsV (AHeap (hb( (Address addr,f_bpl_val) \<mapsto> (val_rel_vpr_bpl v) ))))"
+                             ns (AbsV (AHeap (hb( (Address addr,f_bpl_val) \<mapsto> (val_rel_vpr_bpl v) ))))"
      apply (rule heap_update_wf_apply)
      using  Semantics.RedVar[OF LookupHeapVarBpl]
            apply simp
@@ -458,8 +549,12 @@ proof (rule stmt_rel_intro)
      apply (simp add: NewValTypeBpl)
      done
 
+   have HeapUpdWellTyBpl: "vbpl_absval_ty_opt TyRep (AHeap (hb( (Address addr,f_bpl_val) \<mapsto> (val_rel_vpr_bpl v) ))) = Some (THeapId TyRep, [])"
+     apply (rule heap_upd_ty_preserved[OF HeapWellTyBpl FieldTyBpl])
+     by (simp add: NewValTypeBpl)
+
    have "red_ast_bpl P ctxt 
-           ((BigBlock name (Assign h_bpl h_upd_bpl # cs) str tr, cont), Normal ns3) 
+           ((BigBlock name (Assign h_bpl h_upd_bpl # cs) str tr, cont), Normal ns) 
            ((BigBlock name cs str tr, cont), Normal ?ns_upd)"
      apply (rule red_ast_bpl_one_simple_cmd)
      apply (rule Semantics.RedAssign)
@@ -467,54 +562,10 @@ proof (rule stmt_rel_intro)
      using HeapUpdWellTyBpl \<open>type_interp ctxt = _\<close>
       apply simp
      by (fastforce intro: RedHeapUpdBpl simp: \<open>h_upd_bpl = _\<close>)
-    thus ?thesis
-      using RedNs3 \<open>R \<omega>' ?ns_upd\<close>
-      using red_ast_bpl_transitive by blast      
-  qed
-next
-  let ?Rext = "rel_ext_eq R"
-
-  fix \<omega> ns 
-  assume "R \<omega> ns"
-  hence "?Rext \<omega> \<omega> ns" by simp
-  assume "red_stmt_total ctxt_vpr StateCons \<Lambda>_vpr (FieldAssign rcv_vpr f_vpr rhs_vpr) \<omega> RFailure"
-  thus "\<exists>c'. snd c' = Failure \<and> red_ast_bpl P ctxt (\<gamma>, Normal ns) c'"
-  proof cases
-    case (RedFieldAssignFailure r v)
-    from this obtain ns1 where
-      "?Rext \<omega> \<omega> ns1" and "red_ast_bpl P ctxt (\<gamma>, Normal ns) (\<gamma>1, Normal ns1)"
-      using wf_rel_normal_elim[OF RcvWfRel \<open>?Rext \<omega> \<omega> ns\<close>]
-      by auto      
-    from this RedFieldAssignFailure obtain ns2 where "?Rext \<omega> \<omega> ns2" and "red_ast_bpl P ctxt (\<gamma>, Normal ns) (\<gamma>2, Normal ns2)"
-      using wf_rel_normal_elim[OF RhsWfRel] red_ast_bpl_transitive
-      by blast
-
-    with RedFieldAssignFailure obtain \<gamma>' where "red_ast_bpl P ctxt (\<gamma>, Normal ns) (\<gamma>', Failure)"
-      using wf_rel_failure_elim[OF WriteableLocRel \<open>?Rext \<omega> \<omega> ns2\<close>] red_ast_bpl_transitive
-      by (metis (no_types, opaque_lifting) ref.exhaust ref.sel snd_conv surj_pair)
-    thus ?thesis
-      by (meson snd_conv)
-  next
-    case RedSubExpressionFailure
-    hence RedSubExpFailureAux: "red_pure_exps_total ctxt_vpr StateCons (Some \<omega>) [rcv_vpr, rhs_vpr] \<omega> None"
-      by simp
-    show ?thesis
-    proof (cases  "ctxt_vpr, StateCons, (Some \<omega>) \<turnstile> \<langle>rcv_vpr; \<omega>\<rangle> [\<Down>]\<^sub>t VFailure")
-      case True
-      then show ?thesis 
-        using wf_rel_failure_elim[OF RcvWfRel \<open>?Rext \<omega> \<omega> ns\<close>]
-        by blast
-    next
-      case False
-      from this obtain v where "ctxt_vpr, StateCons, (Some \<omega>) \<turnstile> \<langle>rcv_vpr; \<omega>\<rangle> [\<Down>]\<^sub>t Val v" and
-                               "ctxt_vpr, StateCons, (Some \<omega>) \<turnstile> \<langle>rhs_vpr; \<omega>\<rangle> [\<Down>]\<^sub>t VFailure" 
-        using RedSubExpFailureAux
-        by (auto elim: red_pure_exp_total_elims)
-      then show ?thesis 
-        using wf_rel_normal_elim[OF RcvWfRel \<open>?Rext \<omega> \<omega> ns\<close>] wf_rel_failure_elim[OF RhsWfRel] red_ast_bpl_transitive
-        by blast
-    qed
-  qed
+   thus " \<exists>ns'. red_ast_bpl P ctxt ((BigBlock name (Assign h_bpl h_upd_bpl # cs) str tr, cont), Normal ns) ((BigBlock name cs str tr, cont), Normal ns') \<and> R \<omega>' ns'"
+     using \<open>R \<omega>' ?ns_upd\<close>
+     by blast  
+ qed
 qed
 
 text \<open>Version of generic field assignment relation rule where state relation is instantiated\<close>
@@ -579,7 +630,6 @@ proof (rule field_assign_rel[OF WfConsistency, where ?\<tau>_vpr = "the (declare
                         vbpl_absval_ty_opt TyRep (AHeap hb) = Some (THeapId TyRep, []) \<and>
                         lookup_var (var_context ctxt) ns f_bpl = Some (AbsV (AField f_bpl_val)) \<and>
                         field_ty_fun_opt TyRep f_bpl_val = Some ((TFieldId TyRep), [TConSingle (TNormalFieldId TyRep), \<tau>_bpl]) \<and>
-                        vbpl_absval_ty_opt TyRep (AHeap (hb( (Address addr,f_bpl_val) \<mapsto> (val_rel_vpr_bpl v) ))) = Some (THeapId TyRep, []) \<and>
                         R ?\<omega>' 
                          (update_var (var_context ctxt) ns (heap_var Tr) 
                                (AbsV (AHeap (hb( (Address addr,f_bpl_val) \<mapsto> (val_rel_vpr_bpl v) ))))
@@ -1426,12 +1476,6 @@ abbreviation state_during_inhale_post_call
                                 get_total_full = get_total_full \<omega> \<rparr>"
 
 subsubsection \<open>General lemma\<close>
-
-(*
-declare [[show_types]]
-declare [[show_sorts]]
-declare [[show_consts]]
-*)
 
 lemma method_call_stmt_rel_general:
   assumes MdeclSome:  "program.methods (program_total ctxt_vpr) m = Some mdecl"
